Complexity.lean
@@ -193,6 +193,8 @@ import Complexity.Computability.Ram.Compiler.Language.MeasuredValues
 import Complexity.Computability.Ram.Compiler.Language.Placement
 import Complexity.Computability.Ram.Compiler.Language.Program
 import Complexity.Computability.Ram.Compiler.Language.Program.ArrayFunction
+import Complexity.Computability.Ram.Compiler.Language.Program.ArrayInput
+import Complexity.Computability.Ram.Compiler.Language.Program.Deriving
 import Complexity.Computability.Ram.Compiler.Language.Program.Input
 import Complexity.Computability.Ram.Compiler.Language.Realization
 import Complexity.Computability.Ram.Compiler.Language.Realization.Finite
@@ -457,7 +459,9 @@ import Complexity.Language.Verification.Recursion
 import Complexity.Language.Verification.Tactic
 import Complexity.LinearAlgebra.Matrix.Update
 import Complexity.Program.ArrayFunction
+import Complexity.Program.ArrayInput
 import Complexity.Program.Basic
+import Complexity.Program.Deriving
 import Complexity.Program.Input
 import Complexity.Tactic.Ram.Array
 import Complexity.Tactic.Ram.Basic
